call<->inlined

cancellation/Cancel.v
@@ -55,17 +55,13 @@ Section INTERP.
 
   Definition prog (ms: HModSem.t) : callE ~> itree hmodE :=
     fun _ '(Call fn args) =>
-      (* '(_, body) <- (alist_find fn ms.(HModSem.fnsems))!;; *)
-      (* body args. *)
       lbody <- (alist_find fn ms.(HModSem.fnsems))!;;
       HModSem.sandbox_body lbody args.
-
       
   Definition interp_hpI_fbody (ms: HModSem.t)
     : (list string * (Any.t -> itree hmodE Any.t)) -> (list string * (Any.t -> itree hmodE Any.t))
     :=
     fun '(k, b) => (k, interp_hpI_fun (prog ms) b).
-
 
   Definition wrap_sandbox scopeS: list string * (Any.t -> itree hmodE Any.t) -> list string * (Any.t -> itree hmodE Any.t)
     := 
@@ -75,11 +71,7 @@ Section INTERP.
     :=
     fun kb => interp_hpI_fbody ms (wrap_sandbox ms.(HModSem.scopes) kb). 
 
-
-
 End INTERP.
-
-
 
 
 Module HIRed.
@@ -87,12 +79,13 @@ Module HIRed.
     Context `{Σ: GRA.t}.
 
     Variable ms: HModSem.t.
-    
-    Lemma bisim_iter_handle_bind i k:
+
+    Lemma iter_handle_bind i k:
       ITree.iter (handle_callE (prog ms)) (i >>= k)
-      ≅
+      =
       x <- (ITree.iter (handle_callE (prog ms)) i);; ITree.iter (handle_callE (prog ms)) (k x).
-    Proof.
+    Proof. 
+      eapply bisim_is_eq.
       eapply (@gpaco2_init _ _ _ _ (eqitC eq false false)); eauto with paco.
       revert i k. gcofix CIH. i.
       ides i.
@@ -135,15 +128,6 @@ Module HIRed.
         r. grind. gstep. econs. gbase. eauto.
       Unshelve. eauto with paco.
     Qed.
-
-    Lemma iter_handle_bind i k:
-      ITree.iter (handle_callE (prog ms)) (i >>= k)
-      =
-      x <- (ITree.iter (handle_callE (prog ms)) i);; ITree.iter (handle_callE (prog ms)) (k x).
-    Proof. 
-    Admitted.
-      (* eapply bisim_is_eq. apply bisim_iter_handle_bind. *)
-    (* Qed. *)
         
     Lemma ret 
       prog (x: Any.t)
@@ -227,14 +211,8 @@ End HIRed.
 Section CANCEL.
   Context `{Σ: GRA.t}.
 
-  (* Variable md: HMod.t.
-  Variable ginv: Sk.t -> invspec.
-  Variable stb: Sk.t -> gname -> option fspec.
-
-  Let sk: Sk.t := HMod.sk md. *)
-
-  Definition bindRR {R} Ist CIH : nat -> alist key Any.t * R-> alist key Any.t * R -> iProp :=
-    fun nths '(st0, ret0) '(st1, ret1) => ((⌜ret0 = ret1⌝ ∗ Ist nths st0 st1) ∗ □CIH)%I.
+  Definition bindRR {R} Ist P : nat -> alist key Any.t * R-> alist key Any.t * R -> iProp :=
+    fun nths '(st0, ret0) '(st1, ret1) => (⌜ret0 = ret1⌝ ∗ Ist nths st0 st1 ∗ P)%I.
 
   Definition progI fl : callE ~> itree hmodE :=
     fun _ '(Call fn args) =>
@@ -258,32 +236,44 @@ Section CANCEL.
     rewrite/interp_hpI iter_bind_I. refl.
   Qed.
 
+  Lemma isim_RR_frame
+      fls flt my_tid is_closed r g nths
+      {R} Ist (P: iProp)
+      ps pt sti_src sti_tgt
+    :
+      (P ∗ @isim _ fls flt Ist my_tid is_closed r g R 
+            (fun nths '(sts, vs) '(stt, vt) => ⌜vs = vt⌝ ∗ Ist nths sts stt)%I
+            ps pt nths sti_src sti_tgt)  
+      ⊢ isim fls flt Ist my_tid is_closed r g 
+         (bindRR Ist P) ps pt nths sti_src sti_tgt.
+  Proof.
+    Local Transparent isim.
+    remember (λ (nths0 : nat) '(sts, vs) '(stt, vt), ⌜vs = vt⌝ ∗ Ist nths0 sts stt)%I.
+    uiprop. i. des. subst. rename H1 into SIM. 
+    unfold bindRR.
+    
+  Admitted.
+
 
   Lemma cancelI
-      (* prog *)
       fl my_tid nths
       ps pt
       st_src st_tgt (itr: itree hmodE Any.t)
-      (* scopes *)
-      (* + something about function scopes found in fls, flt *)
     :
     IstEq0 nths st_src st_tgt
     ⊢ isim fl fl IstEq0 my_tid true ibot ibot
        (fun nths '(st_src, v_src) '(st_tgt, v_tgt) => (⌜v_src = v_tgt⌝ ∗ IstEq0 nths st_src st_tgt)%I)
        ps pt nths (st_src, interp_hpI (progI fl) itr) (st_tgt, itr).
-       (* ps pt nths (st_src, interp_hpI (progI fl) (HModSem.sandbox scopes itr)) (st_tgt, (HModSem.sandbox scopes itr)). *)
   Proof.
     revert itr.
-    revert st_tgt. apply combine_quant_dep.
-    revert st_src. apply combine_quant_dep.
-    (* revert scopes. apply combine_quant. *)
-    revert pt. apply combine_quant_dep.
-    revert ps. apply combine_quant_dep.
-    revert nths. apply combine_quant_dep.
+    revert st_tgt. apply combine_quant.
+    revert st_src. apply combine_quant.
+    revert pt. apply combine_quant.
+    revert ps. apply combine_quant.
+    revert nths. apply combine_quant.
     eapply isim_coind. i.
 
     destruct a as [nths [ps [pt [st_src [st_tgt it]]]]]. s.
-    (* destruct a as [nths [ps [pt [scopes [st_src [st_tgt it]]]]]]. s. *)
     iIntros "(#(_ & CIH) & Ist)".
     
     assert (CASE := case_itrH _ it); des; subst.
@@ -301,35 +291,20 @@ Section CANCEL.
     - destruct c. rewrite/__ HIRed.call. steps_l. 
 
       destruct (alist_find fn fl) eqn:FIND; cycle 1.
-      { 
-        (* rewrite/__ HModSB.transl_bind HModSB.transl_call. *)
-        iApply isim_call_none; ss.
-        unfold triggerNB. steps_r. ss.
-      }
+      { iApply isim_call_none; ss. unfold triggerNB. steps_r. ss. }
       iApply isim_inline_tgt; eauto.
       s. ired. rewrite/__ bind_I.
-      remember (∀ a : {_ : nat & {_ : bool & {_ : bool & {_ : alist key Any.t & {_ : alist key Any.t & itree hmodE Any.t}}}}},
-      IstEq0 (projT1 a) (projT1 (projT2 (projT2 (projT2 a)))) (projT1 (projT2 (projT2 (projT2 (projT2 a))))) -∗
-      g0 Any.t (λ (nths0 : nat) '(st_src0, v_src) '(st_tgt0, v_tgt), ⌜v_src = v_tgt⌝ ∗ IstEq0 nths0 st_src0 st_tgt0)
-        (projT1 (projT2 a)) (projT1 (projT2 (projT2 a))) (projT1 a)
-        (projT1 (projT2 (projT2 (projT2 a))), interp_hpI (progI fl) (projT2 (projT2 (projT2 (projT2 (projT2 a))))))
-        (projT1 (projT2 (projT2 (projT2 (projT2 a)))), projT2 (projT2 (projT2 (projT2 (projT2 a))))))%I.
+      remember (
+        ∀ a : nat * (bool * (bool * (alist key Any.t * (alist key Any.t * itree hmodE Any.t)))),
+          IstEq0 a.1 a.2.2.2.1 a.2.2.2.2.1 -∗
+          g0 Any.t (λ (nths0 : nat) '(st_src0, v_src) '(st_tgt0, v_tgt), ⌜v_src = v_tgt⌝ ∗ IstEq0 nths0 st_src0 st_tgt0) a.2.1 a.2.2.1 a.1
+            (a.2.2.2.1, interp_hpI (progI fl) a.2.2.2.2.2) (a.2.2.2.2.1, a.2.2.2.2.2)
+      )%I.
       iApply isim_bind; cycle 1.
       {
         instantiate (1:= (fun nths '(st_src, v_src) '(st_tgt, v_tgt) => (⌜v_src = v_tgt⌝ ∗ IstEq0 nths st_src st_tgt ∗ □b)%I)).
-        (* by_coind "CIH". eauto.   *)
-
-        (* Check (@bindRR Any.t IstEq0 b).  *)
-        rewrite Heqb.
-        (* instantiate (1:= @bindRR Any.t IstEq0 b).  *)
-        iApply isim_progress; iApply isim_base.
-        iSpecialize ("CIH" $! _); repeat instantiate (1:= existT _ _); s.
-        (* unfold bindRR. *)
-        (* iApply "CIH". *)
-        (* instantiate (1:= EqRR ). *)
-        (* by_coind "CIH".   *)
-        (* admit. *)
-        admit.
+        iApply isim_RR_frame. iSplitR; eauto.
+        rewrite Heqb. by_coind "CIH". eauto.
       }
       i. iIntros "(% & IST & #CIH)". des. subst.
       rewrite HIRed.tau. steps_l. steps_r. ired.
@@ -345,16 +320,8 @@ Section CANCEL.
       + steps_l. force_r. instantiate (1:= q).
         by_coind "CIH". auto.
       + step. steps_l. by_coind "CIH". auto.
-    Unshelve. all: eauto.
-  Admitted.
+  Qed.
 
-
-
-   (* Ist nths st_src st_tgt ⊢ *)
-     (* @isim Σ fl_src fl_tgt Ist my_tid is_closed ibot ibot Any.t *)
-     (* (fun nths '(st_src, v_src) '(st_tgt, v_tgt) => (⌜v_src = v_tgt⌝ ∗ Ist nths st_src st_tgt))%I *)
-     (* false false nths (st_src, itr_src) (st_tgt, itr_tgt)))%signature. *)
-    
 End CANCEL.
 
 
@@ -406,50 +373,11 @@ Section CANCEL.
   Context `{Σ: GRA.t}.
 
   Variable md: HMod.t.
-  Variable ginv: Sk.t -> invspec.
-  Variable stb: Sk.t -> gname -> option fspec.
 
   Let sk: Sk.t := HMod.sk md.
-  (* Let ms (sk0: Sk.t) (SKINCL: incl sk sk0) (SKWF: Sk.wf sk0) :=  *)
-    (* HMod.modsem md sk0. *)
-    
-  (* (COND: forall sk0 (EQV: Sk.equiv sk sk0) (SKWF: Sk.wf sk0), 
-  exists fsp m rt,
-    (stb sk0 "CCR_init" = Some fsp) /\
-    (forall rs (WF: URA.wf rs) (SRC: Own rs -∗ (Ps sk0)), URA.wf (rs ⋅ rt)) /\ 
-    (Own rt ⊢ (Pt sk0) ∗ (fsp.(precond) 0 m tt↑ tt↑)) /\
-    (∀ m vret ret, (fsp.(postcond) 0 m vret ret) -∗ ⌜vret = ret⌝)
-) *)
 
-  Lemma alist_find_elimI
-      ms fn fs
-      (FINDS: alist_find fn (HModSem.fnsems (HModSemAux.to_elimI ms)) = Some fs)
-    :
-    exists ft, 
-      fs = interp_hpI_fbody ms (wrap_sandbox (ms.(HModSem.scopes)) ft) /\
-      incl ft.1 ms.(HModSem.scopes)
-      .
-  Proof.
-  Admitted. 
-
-  (* Definition bindRR {R} Ist CIH : nat -> alist key Any.t * R-> alist key Any.t * R -> iProp := *)
-    (* fun nths '(st0, ret0) '(st1, ret1) => ((⌜ret0 = ret1⌝ ∗ Ist nths st0 st1) ∗ □CIH)%I. *)
-
-    (* (⌜v_src = v_tgt⌝ ∗ Ist nths st_src st_tgt))%I *)
-
-
-
-  Lemma cancel0
-    (* scopes fs ft
-    (MAIN: 
-      ∀sk0 (SKINCL: incl (HMod.sk md) sk0) (SKWF: Sk.wf sk0),
-        (alist_find "CRIS_main" (HModSem.fnsems (HModSemAux.to_elimI (HMod.modsem md sk0)))
-          = Some (scopes, fs)) /\
-        (alist_find "CRIS_main" (HModSem.fnsems (HMod.modsem md sk0))
-          = Some (scopes, ft)) /\
-        (fs = interp_hpI_fun (prog (HMod.modsem md sk0)) ft)) *)
+  Lemma cancel_call
   :
-    (* HSimC.t (HModAux.to_elimI md) md IC IstEq. *)
     refines (HModAux.to_elimI md, const(emp%I)) (md, const(emp%I)).
   Proof.
     eapply closed_adequacy.
@@ -460,87 +388,48 @@ Section CANCEL.
     { rewrite map_length. ss. }
     { i. rewrite/__ map_map_compose fst_map_snd in IN. ss. }
     ii. hexploit FIND. i. destruct fs.
-    eapply alist_find_elimI in H. des. exists ft.
-    esplits. { admit. }
-    ii. subst. destruct ft. s in H0.
-    unfold wrap_sandbox, interp_hpI_fbody in H. s in H.
-    inv H. revert H0.
-    generalize (HModSem.scopes (HMod.modsem md sk0)) as scopeS. i.
-    rename l0 into scopeT. rename H0 into INCL.
+
+    unfold HModSemAux.to_elimI in H. s in H.
+    rewrite/__ alist_find_map_snd /o_map in H. des_ifs.
+    rename p into ft. exists ft.
+    esplits; eauto.
+    ii. subst. destruct ft.
+    assert(SCP := (HMod.modsem md sk0).(HModSem.well_scoped_fns)).
+    specialize (SCP fn). rewrite/fnsems_scopes Heq in SCP.
+    remember (HModSem.scopes (HMod.modsem md sk0)) as scopeS. i.
+    rename l into scopeT. 
     unfold HModSem.sandbox_body, interp_hpI_fun. s.
     generalize false at 1 as ps.
     generalize false at 1 as pt. intros pt ps.
-    generalize (i0 y) as it. clear IN fn FIND i0 y.
-
-    (* remember (λ (nths0 : nat) '(st_src, v_src) '(st_tgt0, v_tgt), ⌜v_src = v_tgt⌝ ∗ *)
-    (* IstEq sk0 nths0 st_src st_tgt0)%I as RR. *)
-    revert NODD. apply combine_quant.
-    revert NODS. apply combine_quant.
+    generalize (i y) as it. clear Heq IN fn FIND i y NODD NODS.
     revert st_tgt. apply combine_quant_dep.
     revert st_src. apply combine_quant_dep.
-    revert INCL. apply combine_quant.
+    revert SCP. apply combine_quant.
     revert scopeT. apply combine_quant_dep.
+    revert HeqscopeS. apply combine_quant.
     revert scopeS. apply combine_quant_dep.
-    (* revert HeqRR. apply combine_quant_dep. *)
-    (* revert RR. apply combine_quant_dep. *)
-
-
-    (* revert st_src. apply combine_quant_dep. *)
     revert pt. apply combine_quant.
     revert ps. apply combine_quant.
     revert nths. apply combine_quant.
     eapply isim_coind. i.
 
-    (* unfold HModSem.sandbox. *)
-    (* remember (
-      □ ((∀ (R : Type) (RR : nat → alist key Any.t * R → alist key Any.t * R → iProp) 
-      (ps pt : bool) (nths0 : nat) (src tgt : alist key Any.t * itree hmodE R),
-      ibot RR ps pt nths0 src tgt -∗ g0 R RR ps pt nths0 src tgt) ∗
-   (∀ a0 : nat *
-           {_ : bool &
-           {_ : bool &
-           {_ : list string &
-           (list string *
-            {a3 : list (key * Any.t) &
-            {a4 : list (key * Any.t) &
-            NoDup (List.map fst a3) * (NoDup (List.map fst a4) * itree hmodE Any.t)}})%type}}},
-      IstEq sk0 a0.1 (projT1 (projT2 (projT2 (projT2 a0.2))).2)
-        (projT1 (projT2 (projT2 (projT2 (projT2 a0.2))).2)) -∗
-      g0 Any.t
-        (λ (nths : nat) '(st_src, v_src) '(st_tgt, v_tgt), ⌜v_src = v_tgt⌝ ∗
-           IstEq sk0 nths st_src st_tgt) (projT1 a0.2) (projT1 (projT2 a0.2)) a0.1
-        (projT1 (projT2 (projT2 (projT2 a0.2))).2,
-        translate (HModSem.handle_sandbox (projT1 (projT2 (projT2 a0.2))))
-          (interp_hpI (prog (HMod.modsem md sk0))
-             (projT2 (projT2 (projT2 (projT2 (projT2 a0.2))).2)).2.2))
-        (projT1 (projT2 (projT2 (projT2 (projT2 a0.2))).2),
-        translate (HModSem.handle_sandbox (projT2 (projT2 (projT2 a0.2))).1)
-          (projT2 (projT2 (projT2 (projT2 (projT2 a0.2))).2)).2.2)))
-    )%I. *)
-
-    (* rewrite Heqb. *)
-
-    destruct a as [nths [ps [pt [scopeS [scopeT [INCL [st_src [st_tgt [NODS [NODD it]]]]]]]]]]. s.
+    destruct a as [nths [ps [pt [scopeS [HeqscopeS [scopeT [SCP [st_src [st_tgt it]]]]]]]]]. s.
     iIntros "(#(_ & CIH) & Ist)".
-    
     
     assert (CASE := case_itrH _ it); des; subst.
     - rewrite/__ HModSB.transl_ret HIRed.ret. step. eauto.
     - rewrite/__ HModSB.transl_tau HIRed.tau. steps_l. steps_r. by_coind "CIH". eauto.
-    - rewrite HIRed.bind_ag. steps_l. force_r. iFrame. by_coind "CIH". eauto.
-    - rewrite HIRed.bind_ag. steps_r. force_l. iFrame. steps_l. by_coind "CIH". eauto.
-    - rewrite HIRed.bind_sch. depdes s.
+    - rewrite/__ HModSB.transl_bind HModSB.transl_ag HIRed.bind_ag. steps_l. force_r. iFrame. by_coind "CIH". eauto.
+    - rewrite/__ HModSB.transl_bind HModSB.transl_ag HIRed.bind_ag. steps_r. force_l. iFrame. steps_l. by_coind "CIH". eauto.
+    - rewrite/__ HModSB.transl_bind HModSB.transl_sch HIRed.bind_sch. depdes s.
       + step. steps_l. by_coind "CIH". auto.
       + rewrite/__ !HModSB.transl_bind !HModSB.transl_sch.
         iApply isim_yield. iFrame. iIntros (? ? ? ? ?) "IST".
         steps_l. by_coind "CIH". auto.
       + steps_l. steps_r. by_coind "CIH". auto.
-    - destruct c. rewrite HIRed.call. steps_l. 
-      rewrite/__ HModSB.transl_bind HModSB.transl_call.
-
+    - destruct c. rewrite/__ HModSB.transl_bind HModSB.transl_call HIRed.call. steps_l. 
       destruct (alist_find fn (HModSem.fnsems (HMod.modsem md sk0))) eqn:FIND; cycle 1.
       { 
-        (* rewrite/__ HModSB.transl_bind HModSB.transl_call. *)
         iApply isim_call_none; ss.
         { rewrite/__ alist_find_map_snd FIND. ss. }
         unfold triggerNB. steps_r. ss.
@@ -548,28 +437,154 @@ Section CANCEL.
       destruct p. iApply isim_inline_tgt.
       { rewrite/__ alist_find_map_snd FIND. ss. }
       s. ired. rewrite/__ HIRed.bind HModSB.transl_bind.
+      iStopProof.
+      match goal with
+      | [|-context[(□ ?P)%I]] => remember (□P)%I
+      end.
+      rewrite Heqb. iIntros "[#CIH Ist]". 
       iApply isim_bind; cycle 1.
       {
-        unfold HModSem.sandbox.
-        instantiate (1:= bindRR IstEq0 _).
-        (* instantiate (1:= EqRR ). *)
-        (* by_coind "CIH".   *)
-        admit.
+        instantiate (1:= bindRR IstEq0 b). 
+        iApply isim_RR_frame. rewrite Heqb.  
+        iSplitR; eauto. by_coind "CIH". eauto.  
       }
-      i. iIntros "[[% IST] #CIH]". des. subst.
-      rewrite HIRed.tau. steps_l. steps_r. ired.
-      (* by_coind "CIH". auto. *)
-      admit.
+      i. rewrite Heqb. iIntros "(% & IST & #CIH)". des. subst.
+      rewrite/__ HIRed.tau. steps_l. steps_r. ired.
+      by_coind "CIH". auto.
     - depdes s.
-      + rewrite/__ HIRed.bind_pg !HModSB.transl_bind !HModSB.transl_put. 
-    
-    
-    admit.
-    - rewrite HIRed.bind_core. depdes e.
+      + rewrite/__ !HModSB.transl_bind !HModSB.transl_put. des_ifs; cycle 1. 
+        { steps_r. rewrite HIRed.bind_core. force_l. steps_l. instantiate (1:= q). by_coind "CIH". eauto. }
+        rewrite/__ HIRed.bind_pg HModSB.transl_bind HModSB.transl_put. des_ifs; cycle 1.
+        { 
+          exfalso. eapply existsb_exists in Heq. des. 
+          eapply SCP in Heq. assert (XEQ:= existsb_exists). hdes.
+          rewrite XEQ1 in Heq0; ss; eauto.
+        } 
+        iApply isim_sput_src. iApply isim_sput_tgt.
+        steps_l. by_coind "CIH". iDestruct "Ist" as "%". subst. eauto.
+      + rewrite/__ !HModSB.transl_bind !HModSB.transl_get. des_ifs; cycle 1.
+        { steps_r. rewrite HIRed.bind_core. force_l. steps_l. instantiate (1:= q). by_coind "CIH". eauto. }
+        rewrite/__ HIRed.bind_pg HModSB.transl_bind HModSB.transl_get. des_ifs; cycle 1.
+        { 
+          exfalso. eapply existsb_exists in Heq. des. 
+          eapply SCP in Heq. assert (XEQ:= existsb_exists). hdes.
+          rewrite XEQ1 in Heq0; ss; eauto.
+        } 
+        iApply isim_sget_src. iApply isim_sget_tgt.
+        steps_l. iDestruct "Ist" as "%". subst. 
+        by_coind "CIH". eauto.
+    - rewrite/__ HModSB.transl_bind HModSB.transl_core HIRed.bind_core. depdes e.
       + steps_r. force_l. steps_l.
         instantiate (1:= q). by_coind "CIH". eauto.
       + steps_l. force_r. instantiate (1:= q).
         by_coind "CIH". auto.
       + step. steps_l. by_coind "CIH". auto.
+    Unshelve. all: eauto.
+    {
+      assert(SCP0 := (HMod.modsem md sk0).(HModSem.well_scoped_fns)).
+      specialize (SCP0 fn). rewrite/fnsems_scopes FIND in SCP0. eauto.
+    }
+  Qed.
+      
+  Lemma cancel_call_rev
+  :
+    refines (md, const(emp%I)) (HModAux.to_elimI md, const(emp%I)).
+  Proof.
+    eapply closed_adequacy.
+    instantiate (1:= IstEq).
+    econs; ss. i. r.
+    econs; ss; try refl.
+    { iIntros "_". iPureIntro. ss. }
+    { rewrite map_length. ss. }
+    { i. rewrite/__ map_map_compose fst_map_snd. ss. }
+    ii. exists (wrap_elimI (HMod.modsem md sk0) fs).
+    esplits.
+    { rewrite/__ alist_find_map_snd /o_map. des_ifs. }
+    ii. subst. destruct fs.
+    assert(SCP := (HMod.modsem md sk0).(HModSem.well_scoped_fns)).
+    specialize (SCP fn). rewrite/fnsems_scopes FIND in SCP.
+    remember (HModSem.scopes (HMod.modsem md sk0)) as scopeS. i.
+    rename l into scopeT. 
+    unfold wrap_elimI. s. unfold HModSem.sandbox_body, interp_hpI_fun. s.
+    generalize false at 1 as ps.
+    generalize false at 1 as pt. intros pt ps.
+    generalize (i y) as it. clear IN fn FIND i y NODD NODS.
+    revert st_tgt. apply combine_quant_dep.
+    revert st_src. apply combine_quant_dep.
+    revert SCP. apply combine_quant.
+    revert scopeT. apply combine_quant_dep.
+    revert HeqscopeS. apply combine_quant.
+    revert scopeS. apply combine_quant_dep.
+    revert pt. apply combine_quant.
+    revert ps. apply combine_quant.
+    revert nths. apply combine_quant.
+    eapply isim_coind. i.
+
+    destruct a as [nths [ps [pt [scopeS [HeqscopeS [scopeT [SCP [st_src [st_tgt it]]]]]]]]]. s.
+    iIntros "(#(_ & CIH) & Ist)".
+    
+    assert (CASE := case_itrH _ it); des; subst.
+    - rewrite/__ HModSB.transl_ret HIRed.ret. step. eauto.
+    - rewrite/__ HModSB.transl_tau HIRed.tau. steps_l. steps_r. by_coind "CIH". eauto.
+    - rewrite/__ HModSB.transl_bind HModSB.transl_ag HIRed.bind_ag. steps_l. force_r. iFrame. steps_r. by_coind "CIH". eauto.
+    - rewrite/__ HModSB.transl_bind HModSB.transl_ag HIRed.bind_ag. steps_r. force_l. iFrame. by_coind "CIH". eauto.
+    - rewrite/__ HModSB.transl_bind HModSB.transl_sch HIRed.bind_sch. depdes s.
+      + step. steps_r. by_coind "CIH". auto.
+      + rewrite/__ !HModSB.transl_bind !HModSB.transl_sch.
+        iApply isim_yield. iFrame. iIntros (? ? ? ? ?) "IST".
+        steps_r. by_coind "CIH". auto.
+      + steps_l. steps_r. by_coind "CIH". auto.
+    - destruct c. rewrite/__ HModSB.transl_bind HModSB.transl_call HIRed.call. steps_r. 
+      destruct (alist_find fn (HModSem.fnsems (HMod.modsem md sk0))) eqn:FIND; cycle 1.
+      { s. unfold triggerNB. ired. rewrite HIRed.bind_core. steps_r. ss. }
+      destruct p. iApply isim_inline_src.
+      { rewrite/__ alist_find_map_snd FIND. ss. }
+      s. ired. rewrite/__ HIRed.bind HModSB.transl_bind.
+      iStopProof.
+      match goal with
+      | [|-context[(□ ?P)%I]] => remember (□P)%I
+      end.
+      rewrite Heqb. iIntros "[#CIH Ist]". 
+      iApply isim_bind; cycle 1.
+      {
+        instantiate (1:= bindRR IstEq0 b). 
+        iApply isim_RR_frame. rewrite Heqb.  
+        iSplitR; eauto. by_coind "CIH". eauto.  
+      }
+      i. rewrite Heqb. iIntros "(% & IST & #CIH)". des. subst.
+      rewrite/__ HIRed.tau. steps_l. steps_r. ired.
+      by_coind "CIH". auto.
+    - depdes s.
+      + rewrite/__ !HModSB.transl_bind !HModSB.transl_put. des_ifs; cycle 1. 
+        { rewrite HIRed.bind_core. steps_r. force_l. instantiate (1:= q). by_coind "CIH". eauto. }
+        rewrite/__ HIRed.bind_pg HModSB.transl_bind HModSB.transl_put. des_ifs; cycle 1.
+        { 
+          exfalso. eapply existsb_exists in Heq. des. 
+          eapply SCP in Heq. assert (XEQ:= existsb_exists). hdes.
+          rewrite XEQ1 in Heq0; ss; eauto.
+        } 
+        iApply isim_sput_src. iApply isim_sput_tgt.
+        steps_r. by_coind "CIH". iDestruct "Ist" as "%". subst. eauto.
+      + rewrite/__ !HModSB.transl_bind !HModSB.transl_get. des_ifs; cycle 1.
+        { rewrite HIRed.bind_core. steps_r. force_l. instantiate (1:= q). by_coind "CIH". eauto. }
+        rewrite/__ HIRed.bind_pg HModSB.transl_bind HModSB.transl_get. des_ifs; cycle 1.
+        { 
+          exfalso. eapply existsb_exists in Heq. des. 
+          eapply SCP in Heq. assert (XEQ:= existsb_exists). hdes.
+          rewrite XEQ1 in Heq0; ss; eauto.
+        } 
+        iApply isim_sget_src. iApply isim_sget_tgt.
+        steps_r. iDestruct "Ist" as "%". subst. 
+        by_coind "CIH". eauto.
+    - rewrite/__ HModSB.transl_bind HModSB.transl_core HIRed.bind_core. depdes e.
+      + steps_r. force_l. instantiate (1:= q). by_coind "CIH". eauto.
+      + steps_l. force_r. steps_r. instantiate (1:= q). by_coind "CIH". auto.
+      + step. steps_r. by_coind "CIH". auto.
+    Unshelve. all: try refl; eauto.
+    {
+      assert(SCP0 := (HMod.modsem md sk0).(HModSem.well_scoped_fns)).
+      specialize (SCP0 fn). rewrite/fnsems_scopes FIND in SCP0. eauto.
+    }
+  Qed.
 
 End CANCEL.
